@prefix rdf:  <http://www.w3.org/1999/02/22-rdf-syntax-ns#>.
@prefix rdfs: <http://www.w3.org/2000/01/rdf-schema#>.
@prefix owl:  <http://www.w3.org/2002/07/owl#>.
@prefix xsd:  <http://www.w3.org/2001/XMLSchema#>.
@prefix skos: <http://www.w3.org/2004/02/skos/core#>.
@prefix adlc: <http://example.org/>.

### Ontology Declaration
adlc:
    a               owl:Ontology ;
    rdfs:comment    "Ontology describing decisions issued by Competition Authority."@en ;
    owl:versionInfo "1.0" .

### Classes
adlc:Organization
    a            owl:Class ;
    rdfs:label   "Organization"@en ;
    rdfs:comment "An organization such as a school, NGO, corporation, club, etc." .

adlc:Corporation
    a               owl:Class ;
    rdfs:subClassOf adlc:Organization ;
    rdfs:label      "Corporation"@en ;
    skos:altLabel   "Société"@fr ;
    rdfs:comment    "A business corporation." .

adlc:GovernmentOrganization
    a               owl:Class ;
    rdfs:subClassOf adlc:Organization .

adlc:MinistryEconomyFinance
    a               owl:Class ;
    rdfs:subClassOf adlc:GovernmentOrganization ;
    rdfs:label      "Ministre de l'économie, des finances et de l'industrie"@fr ;
    skos:altLabel   "le ministre"@fr ;
    skos:altLabel   "ministre de l'économie"@fr .

adlc:AdministrativeAuthority
    a               owl:Class ;
    rdfs:subClassOf adlc:Organization ;
    rdfs:label      "Administrative Authority"@en ;
    skos:altLabel   "Autorité administrative"@fr .

adlc:JurisdictionalAuthority
    a               owl:Class ;
    rdfs:subClassOf adlc:Organization ;
    rdfs:label      "Jurisdictional Authority"@en ;
    skos:altLabel   "Autorité juridictionnelle"@fr ;
    skos:altLabel   "Juridiction"@fr ;
    skos:altLabel   "Jurisdiction"@fr ;
    rdfs:comment    "An organization responsible for interpreting and applying the law."@en ;
    skos:note       "Institution de l'État chargée de dire le droit (cf juris-dictio)."@fr ;
    skos:note       "Tribunaux, Cours d'appel, Conseil d'État, Cour de cassation, Cour européenne des droits de l'homme, Cour de justice de l'Union européenne, etc."@fr .

adlc:CompetitionAuthority
    a               owl:Class ;
    rdfs:subClassOf adlc:AdministrativeAuthority ;
    rdfs:label      "Competition Authority"@en ;
    skos:altLabel   "Autorité de la concurrence"@fr ;
    skos:altLabel   "Conseil de la concurrence"@fr ;
    skos:altLabel   "le Conseil"@fr ;
    skos:altLabel   "ADLC"@fr ;
    rdfs:comment    "The organization responsible for investigating and deciding on competition cases." .

adlc:Referral
    a             owl:Class ;
    rdfs:label    "Referral"@en ;
    skos:altLabel "Saisine"@fr ;
    rdfs:comment  "The submission of a case to the Competition Authority for examination." .

adlc:Hearing
    a             owl:Class ;
    rdfs:label    "Hearing"@en ;
    skos:altLabel "Séance"@fr ;
    rdfs:comment  "A meeting where the Competition Authority hears the parties involved in a competition case." .

adlc:Opinion
    a             owl:Class ;
    rdfs:label    "Opinion"@en ;
    skos:altLabel "Avis"@fr ;
    rdfs:comment  "A formal statement issued by the Competition Authority expressing its findings and views on a particular case." .

adlc:Decision
    a             owl:Class ;
    rdfs:label    "Decision"@en ;
    skos:altLabel "Décision"@fr ;
    skos:altLabel "Judgment"@en ;
    skos:altLabel "Jugement"@fr ;
    skos:note     "The identifiers for these decisions follow the pattern n-D-n, where D is the letter D and n is a number. For example, 12-D-01."@en ;
    rdfs:comment  "A formal decision made by the Competition Authority regarding a competition case. When the decision issuer is omitted in the text, it can be assumed that it's been issued by the Competing Authority." .

adlc:InterimMeasure
    a             owl:Class ;
    rdfs:label    "Interim Measure"@en ;
    skos:altLabel "Mesure conservatoire"@fr ;
    rdfs:comment  "A temporary measure taken by the Competition Authority to prevent harm to competition while it investigates a case." .

### Data Properties
adlc:hasDate
    a            owl:DatatypeProperty ;
    rdfs:label   "has date" ;
    rdfs:comment "Associates an entity with a date, indicating when an event occurred or a document was issued." ;
    rdfs:domain  [ owl:unionOf ( adlc:Hearing adlc:Opinion adlc:Decision adlc:InterimMeasure adlc:Referral ) ] ;
    rdfs:range   xsd:date .

adlc:hasIdentifier
    a            owl:DatatypeProperty ;
    rdfs:label   "has number" ;
    rdfs:comment "Associates an entity with a unique identifier or number." ;
    rdfs:domain  [ owl:unionOf ( adlc:Opinion adlc:Decision adlc:InterimMeasure adlc:Referral ) ] ;
    rdfs:range   xsd:string .

adlc:hasName
    a            owl:DatatypeProperty ;
    rdfs:label   "has name" ;
    rdfs:comment "Associates an entity with the name used to refer to it in a text." ;
    rdfs:domain  adlc:Organization ;
    rdfs:range   xsd:string .

adlc:hasParentOrganization
    a             owl:ObjectProperty ;
    rdfs:label    "has parent organization"@en ;
    skos:altLabel "a société mère"@fr ;
    rdfs:comment  "The larger organization that this organization is a sub-organization of, if any."@en ;
    rdfs:domain   adlc:Organization ;
    rdfs:range    adlc:Organization .

### Object Properties
adlc:issues
    a           owl:ObjectProperty ;
    rdfs:label  "issues" ;
    rdfs:comment
                "A relation between the Competition Authority and the formal statements or decisions it releases, such as opinions and judgments." ;
    rdfs:domain adlc:CompetitionAuthority ;
    rdfs:range  [ owl:unionOf ( adlc:Opinion adlc:Decision adlc:InterimMeasure ) ] .

adlc:submits
    a             owl:ObjectProperty ;
    rdfs:label    "submits"@en ;
    skos:altLabel "saisit"@fr ;
    rdfs:comment  "A relation between an organization or an individual that submits a referral for examination." ;
    rdfs:domain   adlc:Organization ;
    rdfs:range    adlc:Referral .

adlc:addresses
    a           owl:ObjectProperty ;
    rdfs:label  "concerne la décision"@fr ;
    rdfs:comment
                "A relation where a Decision addresses issues arising from a Referral, or the execution of another Decision." ;
    rdfs:domain adlc:Decision ;
    rdfs:range  [ owl:unionOf ( adlc:Referral adlc:Decision ) ] .

adlc:isHeardIn
    a             owl:ObjectProperty ;
    rdfs:label    "is heard"@en ;
    skos:altLabel "est entendu"@fr ;
    rdfs:comment  "A relation between a party and a Hearing, indicating that the party participated in the Hearing." ;
    rdfs:domain   adlc:Organization ;
    rdfs:range    adlc:Hearing .

adlc:precedes
    a           owl:ObjectProperty ;
    rdfs:label  "precedes decision"@en ;
    rdfs:comment
                "A relation between a Hearing and a Decision indicating that the Hearing occurs before and leads up to the Decision."@en ;
    rdfs:domain adlc:Hearing ;
    rdfs:range  adlc:Decision .
